progress proof completed

progress.lean
@@ -1,7 +1,7 @@
 import .syntax .notations .logic .evaluation .vcgen
 
 @[reducible]
-def is_return(s: stack): Prop := ∃(σ: env) (x: var), s = (σ, exp.return x)
+def is_value(s: stack): Prop := ∃(σ: env) (x: var) (v: value), s = (σ, exp.return x) ∧ (σ x = v)
 
 lemma exp.vcgen.return.inv {P: prop} {x: var} {Q: propctx}: (P ⊢ exp.return x : Q) → x ∈ FV P :=
   assume return_verified: P ⊢ exp.return x : Q,
@@ -21,566 +21,159 @@ lemma stack.vcgen.top.inv {H: list call} {σ: env} {e: exp}: (H ⊩ (σ, e)) →
     }
   end
 
+lemma not_free_of_subst_env_val {P: prop} {σ: env} {x y: var} {v: value}:
+       free_in_prop x (P && (y ≡ v)) → (free_in_prop x P → ∀ (R : spec), ¬free_in_prop x ↑(spec.subst_env σ R)) →
+       ∀R: spec, ¬(free_in_prop x (spec.subst_env (σ[y↦v]) R)) :=
+  assume x_free_in_P: free_in_prop x (P && (y ≡ v)),
+  assume ih: free_in_prop x P → ∀ (R : spec), ¬free_in_prop x ↑(spec.subst_env σ R),
+  assume R: spec,
+  assume x_free_in_subst: free_in_prop x (spec.subst_env (σ[y↦v]) R),
+  have x_neq_y: x ≠ y, from (free_of_subst_env_spec x_free_in_subst).left,
+  have free_in_prop x P ∨ free_in_prop x (y ≡ v), from free_in_prop.and.inv x_free_in_P,
+  or.elim this (
+    assume : free_in_prop x P,
+    have x_free_in_R: free_in_prop x (spec.subst_env σ R), from (free_of_subst_env_spec x_free_in_subst).right,
+    have ¬free_in_prop x (spec.subst_env σ R), from ih this R,
+    show «false», from this x_free_in_R
+  ) (
+    assume : free_in_prop x (y ≡ v),
+    have free_in_term x (y ≡ v), from free_in_prop.term.inv this,
+    (free_in_term.binop.inv this).elim (
+      assume : free_in_term x y,
+      have x = y, from free_in_term.var.inv this,
+      show «false», from x_neq_y this
+    ) (
+      assume : free_in_term x v,
+      show «false», from free_in_term.value.inv this
+    )
+  )
+
 lemma not_free_of_subst_env {P: prop} {σ: env} {x: var}:
        (⊢ σ : P) → free_in_prop x P → ∀R: spec, ¬(free_in_prop x (spec.subst_env σ R)) :=
-  sorry
-  -- assume env_verified: ⊢ σ : P,
-  -- assume x_free_in_P: free_in_prop x P,
-  -- show (∀R: spec, ¬(free_in_prop x (spec.subst_env σ R))), by begin
-  --   induction env_verified,
-  --   case env.vcgen.empty { from
-  --     assume R: spec,
-  --     assume x_free_in_subst: free_in_prop x (spec.subst_env env.empty R),
-  --     have free_in_term x value.true, from free_in_prop.term.inv x_free_in_P,
-  --     show «false», from free_in_term.value.inv this
-  --   },
-  --   case env.vcgen.tru σ' y Q _ _ ih { from
-  --     assume R: spec,
-  --     assume x_free_in_subst: free_in_prop x (spec.subst_env (σ'[y↦value.true]) R),
-  --     have x_neq_y: x ≠ y, from (free_of_subst_env_spec x_free_in_subst).left,
-  --     have free_in_prop x Q ∨ free_in_prop x (y ≡ value.true), from free_in_prop.and.inv x_free_in_P,
-  --     or.elim this (
-  --       assume : free_in_prop x Q,
-  --       have x_free_in_R: free_in_prop x (spec.subst_env σ' R), from (free_of_subst_env_spec x_free_in_subst).right,
-  --       have ¬free_in_prop x (spec.subst_env σ' R), from ih this R,
-  --       show «false», from this x_free_in_R
-  --     ) (
-  --       assume : free_in_prop x (y ≡ value.true),
-  --       have free_in_term x (y ≡ value.true), from free_in_prop.term.inv this,
-  --       (free_in_term.binop.inv this).elim (
-  --         assume : free_in_term x y,
-  --         have x = y, from free_in_term.var.inv this,
-  --         show «false», from x_neq_y this
-  --       ) (
-  --         assume : free_in_term x (value.true),
-  --         show «false», from free_in_term.value.inv this
-  --       )
-  --     )
-  --   },
-  --   case env.vcgen.fls σ' y Q _ _ ih { from
-  --     assume R: spec,
-  --     assume x_free_in_subst: free_in_prop x (spec.subst_env (σ'[y↦value.false]) R),
-  --     have x_neq_y: x ≠ y, from (free_of_subst_env_spec x_free_in_subst).left,
-  --     have free_in_prop x Q ∨ free_in_prop x (y ≡ value.false), from free_in_prop.and.inv x_free_in_P,
-  --     or.elim this (
-  --       assume : free_in_prop x Q,
-  --       have x_free_in_R: free_in_prop x (spec.subst_env σ' R), from (free_of_subst_env_spec x_free_in_subst).right,
-  --       have ¬free_in_prop x (spec.subst_env σ' R), from ih this R,
-  --       show «false», from this x_free_in_R
-  --     ) (
-  --       assume : free_in_prop x (y ≡ value.false),
-  --       have free_in_term x (y ≡ value.false), from free_in_prop.term.inv this,
-  --       (free_in_term.binop.inv this).elim (
-  --         assume : free_in_term x y,
-  --         have x = y, from free_in_term.var.inv this,
-  --         show «false», from x_neq_y this
-  --       ) (
-  --         assume : free_in_term x (value.false),
-  --         show «false», from free_in_term.value.inv this
-  --       )
-  --     )
-  --   },
-  --   case env.vcgen.num n σ' y Q _ _ ih { from
-  --     assume R: spec,
-  --     assume x_free_in_subst: free_in_prop x (spec.subst_env (σ'[y↦value.num n]) R),
-  --     have x_neq_y: x ≠ y, from (free_of_subst_env_spec x_free_in_subst).left,
-  --     have free_in_prop x Q ∨ free_in_prop x (y ≡ value.num n), from free_in_prop.and.inv x_free_in_P,
-  --     or.elim this (
-  --       assume : free_in_prop x Q,
-  --       have x_free_in_R: free_in_prop x (spec.subst_env σ' R), from (free_of_subst_env_spec x_free_in_subst).right,
-  --       have ¬free_in_prop x (spec.subst_env σ' R), from ih this R,
-  --       show «false», from this x_free_in_R
-  --     ) (
-  --       assume : free_in_prop x (y ≡ value.num n),
-  --       have free_in_term x (y ≡ value.num n), from free_in_prop.term.inv this,
-  --       (free_in_term.binop.inv this).elim (
-  --         assume : free_in_term x y,
-  --         have x = y, from free_in_term.var.inv this,
-  --         show «false», from x_neq_y this
-  --       ) (
-  --         assume : free_in_term x (value.num n),
-  --         show «false», from free_in_term.value.inv this
-  --       )
-  --     )
-  --   },
-  --   case env.vcgen.func f σ₁ σ₂ g gx R' S' e Q₁ Q₂ Q₃ _ _ _ fv_R fv_S _ _ ih₁ ih₂ { from
-  --     assume R: spec,
-  --     assume x_free_in_subst: free_in_prop x (spec.subst_env (σ₂[f↦value.func g gx R' S' e σ₁]) R),
-  --     have x_neq_f: x ≠ f, from (free_of_subst_env_spec x_free_in_subst).left,
-  --     let R'' := spec.subst_env (σ₁[g↦value.func g gx R' S' e σ₁]) R' in
-  --     let S'' := spec.subst_env (σ₁[g↦value.func g gx R' S' e σ₁]) S' in
-  --     have free_in_prop x (Q₁ && spec.func ↑f gx R'' S'') ∨ free_in_prop x (f ≡ value.func g gx R' S' e σ₁),
-  --     from free_in_prop.and.inv x_free_in_P,
-  --     or.elim this (
-  --       assume : free_in_prop x (Q₁ && spec.func f gx R'' S''),
-  --       or.elim (free_in_prop.and.inv this) (
-  --         assume : free_in_prop x Q₁,
-  --         have x_free_in_R: free_in_prop x (spec.subst_env σ₂ R), from (free_of_subst_env_spec x_free_in_subst).right,
-  --         have ¬free_in_prop x (spec.subst_env σ₂ R), from ih₁ this R,
-  --         show «false», from this x_free_in_R
-  --       ) (
-  --         assume x_free_in_func: free_in_prop x (spec.func f gx R'' S''),
-  --         let forallp := (prop.implies R''.to_prop (prop.pre f gx)
-  --                       && prop.implies (R''.to_prop && prop.post f gx) S''.to_prop) in
-  --         have h: (spec.func f gx R'' S'').to_prop = (term.unop unop.isFunc f && prop.forallc gx f forallp),
-  --         by unfold spec.to_prop,
-  --         have free_in_prop x (term.unop unop.isFunc f && prop.forallc gx f forallp), from h ▸ x_free_in_func,
-  --         have free_in_prop x (term.unop unop.isFunc f) ∨ free_in_prop x (prop.forallc gx f forallp),
-  --         from free_in_prop.and.inv this,
-  --         or.elim this (
-  --           assume : free_in_prop x (term.unop unop.isFunc f),
-  --           have free_in_term x (term.unop unop.isFunc f), from free_in_prop.term.inv this,
-  --           have free_in_term x f, from free_in_term.unop.inv this,
-  --           have x = f, from free_in_term.var.inv this,
-  --           show «false», from x_neq_f this
-  --         ) (
-  --           assume : free_in_prop x (prop.forallc gx f forallp),
-  --           have x_neq_gx: x ≠ gx, from (free_in_prop.forallc.inv this).left,
-  --           have free_in_term x f ∨ free_in_prop x forallp, from (free_in_prop.forallc.inv this).right,
-  --           or.elim this (
-  --             assume : free_in_term x f,
-  --             have x = f, from free_in_term.var.inv this,
-  --             show «false», from x_neq_f this
-  --           ) (
-  --             assume : free_in_prop x forallp,
-  --             or.elim (free_in_prop.and.inv this) (
-  --               assume : free_in_prop x (prop.implies R''.to_prop (prop.pre f gx)),
-  --               or.elim (free_in_prop.implies.inv this) (
-  --                 assume : free_in_prop x R''.to_prop,
-  --                 have x ≠ g ∧ free_in_prop x (spec.subst_env σ₁ R').to_prop, from free_of_subst_env_spec this,
-  --                 have x_neq_g: x ≠ g, from this.left,
-  --                 have x_free_in_sR': free_in_prop x (spec.subst_env σ₁ R').to_prop, from this.right,
-  --                 have x_free_in_R': x ∈ FV R'.to_prop, from free_of_subst_env x_free_in_sR',
-  --                 have x ∈ FV Q₂ ∪ {g, gx}, from set.mem_of_mem_of_subset x_free_in_R' fv_R,
-  --                 have x ∈ FV Q₂ ∨ x ∈ {g, gx}, from set.mem_or_mem_of_mem_union this,
-  --                 or.elim this (
-  --                   assume : x ∈ FV Q₂,
-  --                   have ¬ free_in_prop x ↑(spec.subst_env σ₁ R'), from ih₂ this R',
-  --                   show «false», from this x_free_in_sR'
-  --                 ) (
-  --                   assume : x ∈ {g, gx},
-  --                   have (x = g) ∨ (x = gx), from mem_of_2set this,
-  --                   or.elim this (
-  --                     assume : x = g,
-  --                     show «false», from x_neq_g this
-  --                   ) (
-  --                     assume : x = gx,
-  --                     show «false», from x_neq_gx this
-  --                   )
-  --                 )
-  --               ) (
-  --                 assume : free_in_prop x (prop.pre f gx),
-  --                 have free_in_term x f ∨ free_in_term x gx, from free_in_prop.pre.inv this,
-  --                 or.elim this (
-  --                   assume : free_in_term x f,
-  --                   have x = f, from free_in_term.var.inv this,
-  --                   show «false», from x_neq_f this
-  --                 ) (
-  --                   assume : free_in_term x gx,
-  --                   have x = gx, from free_in_term.var.inv this,
-  --                   show «false», from x_neq_gx this
-  --                 )
-  --               )
-  --             ) (
-  --               assume : free_in_prop x (prop.implies (R''.to_prop && prop.post f gx) S''.to_prop),
-  --               or.elim (free_in_prop.implies.inv this) (
-  --                 assume : free_in_prop x (R''.to_prop && prop.post f gx),
-  --                 or.elim (free_in_prop.and.inv this) (
-  --                   assume : free_in_prop x R''.to_prop,
-  --                   have x ≠ g ∧ free_in_prop x (spec.subst_env σ₁ R').to_prop, from free_of_subst_env_spec this,
-  --                   have x_neq_g: x ≠ g, from this.left,
-  --                   have x_free_in_sR': free_in_prop x (spec.subst_env σ₁ R').to_prop, from this.right,
-  --                   have x_free_in_R': x ∈ FV R'.to_prop, from free_of_subst_env x_free_in_sR',
-  --                   have x ∈ FV Q₂ ∪ {g, gx}, from set.mem_of_mem_of_subset x_free_in_R' fv_R,
-  --                   have x ∈ FV Q₂ ∨ x ∈ {g, gx}, from set.mem_or_mem_of_mem_union this,
-  --                   or.elim this (
-  --                     assume : x ∈ FV Q₂,
-  --                     have ¬ free_in_prop x ↑(spec.subst_env σ₁ R'), from ih₂ this R',
-  --                     show «false», from this x_free_in_sR'
-  --                   ) (
-  --                     assume : x ∈ {g, gx},
-  --                     have (x = g) ∨ (x = gx), from mem_of_2set this,
-  --                     or.elim this (
-  --                       assume : x = g,
-  --                       show «false», from x_neq_g this
-  --                     ) (
-  --                       assume : x = gx,
-  --                       show «false», from x_neq_gx this
-  --                     )
-  --                   )
-  --                 ) (
-  --                   assume : free_in_prop x (prop.post f gx),
-  --                   have free_in_term x f ∨ free_in_term x gx, from free_in_prop.post.inv this,
-  --                   or.elim this (
-  --                     assume : free_in_term x f,
-  --                     have x = f, from free_in_term.var.inv this,
-  --                     show «false», from x_neq_f this
-  --                   ) (
-  --                     assume : free_in_term x gx,
-  --                     have x = gx, from free_in_term.var.inv this,
-  --                     show «false», from x_neq_gx this
-  --                   )
-  --                 )
-  --               ) (
-  --                 assume : free_in_prop x S''.to_prop,
-  --                 have x ≠ g ∧ free_in_prop x (spec.subst_env σ₁ S').to_prop, from free_of_subst_env_spec this,
-  --                 have x_neq_g: x ≠ g, from this.left,
-  --                 have x_free_in_sS': free_in_prop x (spec.subst_env σ₁ S').to_prop, from this.right,
-  --                 have x_free_in_S': x ∈ FV S'.to_prop, from free_of_subst_env x_free_in_sS',
-  --                 have x ∈ FV Q₂ ∪ {g, gx}, from set.mem_of_mem_of_subset x_free_in_S' fv_S,
-  --                 have x ∈ FV Q₂ ∨ x ∈ {g, gx}, from set.mem_or_mem_of_mem_union this,
-  --                 or.elim this (
-  --                   assume : x ∈ FV Q₂,
-  --                   have ¬ free_in_prop x ↑(spec.subst_env σ₁ S'), from ih₂ this S',
-  --                   show «false», from this x_free_in_sS'
-  --                 ) (
-  --                   assume : x ∈ {g, gx},
-  --                   have (x = g) ∨ (x = gx), from mem_of_2set this,
-  --                   or.elim this (
-  --                     assume : x = g,
-  --                     show «false», from x_neq_g this
-  --                   ) (
-  --                     assume : x = gx,
-  --                     show «false», from x_neq_gx this
-  --                   )
-  --                 )
-  --               )
-  --             )
-  --           )
-  --         )
-  --       )
-  --     ) (
-  --       assume : free_in_prop x (f ≡ value.func g gx R' S' e σ₁),
-  --       have free_in_term x (f ≡ value.func g gx R' S' e σ₁), from free_in_prop.term.inv this,
-  --       (free_in_term.binop.inv this).elim (
-  --         assume : free_in_term x f,
-  --         have x = f, from free_in_term.var.inv this,
-  --         show «false», from x_neq_f this
-  --       ) (
-  --         assume : free_in_term x (value.func g gx R' S' e σ₁),
-  --         show «false», from free_in_term.value.inv this
-  --       )
-  --     )
-  --   }
-  -- end
-  
+  assume env_verified: ⊢ σ : P,
+  assume x_free_in_P: free_in_prop x P,
+  show (∀R: spec, ¬(free_in_prop x (spec.subst_env σ R))), by begin
+    induction env_verified,
+    case env.vcgen.empty { from
+      assume R: spec,
+      assume x_free_in_subst: free_in_prop x (spec.subst_env env.empty R),
+      have free_in_term x value.true, from free_in_prop.term.inv x_free_in_P,
+      show «false», from free_in_term.value.inv this
+    },
+    case env.vcgen.tru σ' y Q _ _ ih {
+      show ∀R: spec, ¬(free_in_prop x (spec.subst_env (σ'[y↦value.true]) R)),
+      from not_free_of_subst_env_val x_free_in_P ih
+    },
+    case env.vcgen.fls σ' y Q _ _ ih { from
+      show ∀R: spec, ¬(free_in_prop x (spec.subst_env (σ'[y↦value.false]) R)),
+      from not_free_of_subst_env_val x_free_in_P ih
+    },
+    case env.vcgen.num n σ' y Q _ _ ih { from
+      show ∀R: spec, ¬(free_in_prop x (spec.subst_env (σ'[y↦value.num n]) R)),
+      from not_free_of_subst_env_val x_free_in_P ih
+    },
+    case env.vcgen.func f σ₁ σ₂ g gx R' S' e Q₁ Q₂ Q₃ _ _ _ fv_R fv_S _ _ ih₁ ih₂ { from
+      show ∀R: spec, ¬(free_in_prop x (spec.subst_env (σ₂[f↦value.func g gx R' S' e σ₁]) R)),
+      from not_free_of_subst_env_val x_free_in_P ih₁
+    }
+  end
 
 lemma val_of_free_in_nonempty_env {P: prop} {σ: env} {x y: var} {v: value}:
-                                  (⊢ σ : P) → (x ≠ y → ∃v', σ y = some v') →
-                                  ∃v', σ[x↦v] y = some v' :=
-  sorry
-  -- assume env_verified: ⊢ σ : P,
-  -- assume ih: x ≠ y → ∃v', σ y = some v',
-  -- if x_eq_y: x = y ∧ option.is_none (σ.apply y) then (
-  --   have h: σ[x↦v].apply x = (if x = x ∧ option.is_none (σ.apply x) then ↑v else σ.apply x), by unfold env.apply,
-  --   have (if x = x ∧ option.is_none (σ.apply x) then ↑v else σ.apply x) = ↑v, by simp *,
-  --   have σ[x↦v].apply x = ↑v, from this ▸ h,
-  --   have σ[x↦v].apply y = some v, from x_eq_y.left ▸ this,
-  --   show ∃v', σ[x↦v] y = some v', from exists.intro v this
-  -- ) else (
-  --   have ∃v', σ y = some v', from (
-  --     have ¬(x = y) ∨ ¬(option.is_none (σ.apply y)), from not_and_distrib.mp x_eq_y,
-  --     this.elim (
-  --       assume : x ≠ y,
-  --       show ∃v', σ y = some v', from ih this        
-  --     ) ( 
-  --       assume : ¬(option.is_none (env.apply σ y)),
-  --       have ¬(option.is_none (σ y)), from this,
-  --       show ∃v', σ y = some v', from not_is_none.rinv.mpr this
-  --     )
-  --   ),
-  --   let ⟨v', σ_has_y⟩ := this in
-  --   have h: σ[x↦v].apply y = (if x = y ∧ option.is_none (σ.apply y) then ↑v else σ.apply y), by unfold env.apply,
-  --   have (if x = y ∧ option.is_none (σ.apply y) then ↑v else σ.apply y) = σ.apply y, by simp *,
-  --   have σ[x↦v].apply y = σ.apply y, from this ▸ h,
-  --   have σ[x↦v].apply y = some v', from eq.trans this σ_has_y,
-  --   show ∃v', σ[x↦v] y = some v', from exists.intro v' this
-  -- )
+                                  (⊢ σ : P) → (x ≠ y → ∃v', σ y = some v') → ∃v', σ[x↦v] y = some v' :=
+  assume env_verified: ⊢ σ : P,
+  assume ih: x ≠ y → ∃v', σ y = some v',
+  if x_eq_y: x = y ∧ option.is_none (σ.apply y) then (
+    have h: σ[x↦v].apply x = (if x = x ∧ option.is_none (σ.apply x) then ↑v else σ.apply x), by unfold env.apply,
+    have (if x = x ∧ option.is_none (σ.apply x) then ↑v else σ.apply x) = ↑v, by simp *,
+    have σ[x↦v].apply x = ↑v, from this ▸ h,
+    have σ[x↦v].apply y = some v, from x_eq_y.left ▸ this,
+    show ∃v', σ[x↦v] y = some v', from exists.intro v this
+  ) else (
+    have ∃v', σ y = some v', from (
+      have ¬(x = y) ∨ ¬(option.is_none (σ.apply y)), from not_and_distrib.mp x_eq_y,
+      this.elim (
+        assume : x ≠ y,
+        show ∃v', σ y = some v', from ih this        
+      ) ( 
+        assume : ¬(option.is_none (env.apply σ y)),
+        have ¬(option.is_none (σ y)), from this,
+        show ∃v', σ y = some v', from not_is_none.rinv.mpr this
+      )
+    ),
+    let ⟨v', σ_has_y⟩ := this in
+    have h: σ[x↦v].apply y = (if x = y ∧ option.is_none (σ.apply y) then ↑v else σ.apply y), by unfold env.apply,
+    have (if x = y ∧ option.is_none (σ.apply y) then ↑v else σ.apply y) = σ.apply y, by simp *,
+    have σ[x↦v].apply y = σ.apply y, from this ▸ h,
+    have σ[x↦v].apply y = some v', from eq.trans this σ_has_y,
+    show ∃v', σ[x↦v] y = some v', from exists.intro v' this
+  )
+
+lemma val_of_free_in_env_value {P: prop} {σ: env} {x y: var} {v: value}:
+  (⊢ σ : P) → x ∈ FV (P && (y ≡ v)) → (x ∈ FV P → (∃ (v : value), σ x = some v)) → ∃v', σ[y↦v] x = some v' :=
+  assume σ_verified: ⊢ σ : P,
+  assume x_free_in_P: x ∈ FV (P && (y ≡ v)),
+  assume ih : x ∈ FV P → (∃ (v : value), σ x = some v),
+  val_of_free_in_nonempty_env σ_verified (
+    assume x'_is_not_x: y ≠ x,
+    have free_in_prop x P ∨ free_in_prop x (y ≡ v), from free_in_prop.and.inv x_free_in_P,
+    or.elim this.symm
+    (
+      assume x_free_in_eq_v: free_in_prop x (y ≡ v),
+      show ∃v', σ x = some v', by begin
+        cases x_free_in_eq_v,
+        case free_in_prop.term x_free_in_eq {
+          cases x_free_in_eq,
+          case free_in_term.binop₁ free_in_y {
+            have y_is_x: (y = x), from (free_in_term.var.inv free_in_y).symm,
+            contradiction
+          },
+          case free_in_term.binop₂ free_in_v {
+            cases free_in_v
+          }
+        }
+      end
+    )
+    (
+      assume x_free_in_P: free_in_prop x P,
+      show ∃v', σ x = some v', from ih x_free_in_P
+    )
+  )
 
 lemma val_of_free_in_env {P: prop} {σ: env} {x: var}: (⊢ σ : P) → x ∈ FV P → ∃v, σ x = some v :=
-  sorry
-  -- assume env_verified: ⊢ σ: P,
-  -- assume x_free_in_P: x ∈ FV P,
-  -- begin
-  --   induction env_verified,
-  --   case env.vcgen.empty {
-  --     cases x_free_in_P,
-  --     case free_in_prop.term x_free_in_true {
-  --       cases x_free_in_true
-  --     }
-  --   },
-  --   case env.vcgen.tru σ' x' Q _ σ'_verified ih { from
-  --     val_of_free_in_nonempty_env σ'_verified (
-  --       assume x'_is_not_x: x' ≠ x,
-  --       have free_in_prop x Q ∨ free_in_prop x (x' ≡ value.true), from free_in_prop.and.inv x_free_in_P,
-  --       or.elim this.symm
-  --       (
-  --         assume x_free_in_true: free_in_prop x (x' ≡ value.true),
-  --         show ∃v, σ' x = some v, by begin
-  --           cases x_free_in_true,
-  --           case free_in_prop.term x_free_in_eq {
-  --             cases x_free_in_eq,
-  --             case free_in_term.binop₁ free_in_x' {
-  --               have x'_is_x: (x' = x), from (free_in_term.var.inv free_in_x').symm,
-  --               contradiction
-  --             },
-  --             case free_in_term.binop₂ free_in_true {
-  --               cases free_in_true
-  --             }
-  --           }
-  --         end
-  --       )
-  --       (
-  --         assume x_free_in_Q: free_in_prop x Q,
-  --         show ∃v, σ' x = some v, from ih x_free_in_Q
-  --       )
-  --     )
-  --   },
-  --   case env.vcgen.fls σ' x' Q _ σ'_verified ih { from
-  --     val_of_free_in_nonempty_env σ'_verified (
-  --       assume x'_is_not_x: x' ≠ x,
-  --       have free_in_prop x Q ∨ free_in_prop x (x' ≡ value.false), from free_in_prop.and.inv x_free_in_P,
-  --       or.elim this.symm
-  --       (
-  --         assume x_free_in_false: free_in_prop x (x' ≡ value.false),
-  --         show ∃v, σ' x = some v, by begin
-  --           cases x_free_in_false,
-  --           case free_in_prop.term x_free_in_eq {
-  --             cases x_free_in_eq,
-  --             case free_in_term.binop₁ free_in_x' {
-  --               have x'_is_x: (x' = x), from (free_in_term.var.inv free_in_x').symm,
-  --               contradiction
-  --             },
-  --             case free_in_term.binop₂ free_in_false {
-  --               cases free_in_false
-  --             }
-  --           }
-  --         end
-  --       )
-  --       (
-  --         assume x_free_in_Q: free_in_prop x Q,
-  --         show ∃v, σ' x = some v, from ih x_free_in_Q
-  --       )
-  --     )
-  --   },
-  --   case env.vcgen.num n σ' x' Q _ σ'_verified ih { from
-  --     val_of_free_in_nonempty_env σ'_verified (
-  --       assume x'_is_not_x: x' ≠ x,
-  --       have free_in_prop x Q ∨ free_in_prop x (x' ≡ value.num n), from free_in_prop.and.inv x_free_in_P,
-  --       or.elim this.symm
-  --       (
-  --         assume x_free_in_num: free_in_prop x (x' ≡ value.num n),
-  --         show ∃v, σ' x = some v, by begin
-  --           cases x_free_in_num,
-  --           case free_in_prop.term x_free_in_eq {
-  --             cases x_free_in_eq,
-  --             case free_in_term.binop₁ free_in_x' {
-  --               have x'_is_x: (x' = x), from (free_in_term.var.inv free_in_x').symm,
-  --               contradiction
-  --             },
-  --             case free_in_term.binop₂ free_in_num {
-  --               cases free_in_num
-  --             }
-  --           }
-  --         end
-  --       )
-  --       (
-  --         assume x_free_in_Q: free_in_prop x Q,
-  --         show ∃v, σ' x = some v, from ih x_free_in_Q
-  --       )
-  --     )
-  --   },
-  --   case env.vcgen.func σ₁ σ₂ f g fx R S e Q₁ Q₂ Q₃ _ σ₁_verified σ₂_verified R_fv S_fv func_verified S_valid { from
-  --     val_of_free_in_nonempty_env σ₁_verified (
-  --       assume f_is_not_x: f ≠ x,
-  --       let R': spec := spec.subst_env (σ₂[g↦value.func g fx R S e σ₂]) R in
-  --       let S': spec := spec.subst_env (σ₂[g↦value.func g fx R S e σ₂]) S in
-  --       let fspec: prop := spec.func f fx R' S' in
-  --       have free_in_prop x (Q₁ && fspec) ∨ free_in_prop x (f ≡ value.func g fx R S e σ₂),
-  --       from free_in_prop.and.inv x_free_in_P,
-  --       or.elim this
-  --       (
-  --         assume : free_in_prop x (Q₁ && fspec),
-  --         have free_in_prop x Q₁ ∨ free_in_prop x fspec, from free_in_prop.and.inv this,
-  --         or.elim this
-  --         (
-  --           assume : free_in_prop x Q₁,
-  --           show ∃v, σ₁ x = some v, from ih_1 this
-  --         )
-  --         (
-  --           assume : free_in_prop x fspec,
-  --           have 
-  --             free_in_prop x (term.unop unop.isFunc f) ∨
-  --             free_in_prop x (prop.forallc fx f (prop.implies R'.to_prop (prop.pre f fx)
-  --                             && prop.implies (R'.to_prop && prop.post f fx) S'.to_prop)),
-  --           from free_in_prop.and.inv this,
-  --           or.elim this
-  --           (
-  --             assume x_free_in_unopp: free_in_prop x (term.unop unop.isFunc f),
-  --             show ∃v, σ₁ x = some v, by begin
-  --               cases x_free_in_unopp,
-  --               case free_in_prop.term x_free_in_unop {
-  --                 cases x_free_in_unop,
-  --                 case free_in_term.unop free_in_f {
-  --                   have : (f = x), from (free_in_term.var.inv free_in_f).symm,
-  --                   contradiction
-  --                 }
-  --               }
-  --             end
-  --           )
-  --           (
-  --             assume : free_in_prop x (prop.forallc fx f (prop.implies R'.to_prop (prop.pre f fx)
-  --                                    && prop.implies (R'.to_prop && prop.post f fx) S'.to_prop)),
-  --             show ∃v, σ₁ x = some v, by begin
-  --               cases this,
-  --               case free_in_prop.forallc₁ x_not_fx x_free_in_f {
-  --                 have : (f = x), from (free_in_term.var.inv x_free_in_f).symm,
-  --                 contradiction
-  --               },
-  --               case free_in_prop.forallc₂ x_neq_fx x_free_in_p { from
-  --                 have free_in_prop x (prop.implies R'.to_prop (prop.pre f fx))
-  --                    ∨ free_in_prop x (prop.implies (R'.to_prop && prop.post f fx) S'.to_prop),
-  --                 from free_in_prop.and.inv x_free_in_p,
-  --                 or.elim this
-  --                 (
-  --                   assume : free_in_prop x (prop.implies R'.to_prop (prop.pre f fx)),
-  --                   have free_in_prop x (prop.or R'.to_prop.not (prop.pre f fx)), from this,
-  --                   have free_in_prop x R'.to_prop.not ∨ free_in_prop x (prop.pre f fx),
-  --                   from free_in_prop.or.inv this,
-  --                   or.elim this
-  --                   (
-  --                     assume : free_in_prop x R'.to_prop.not,
-  --                     have free_in_prop x R'.to_prop, from free_in_prop.not.inv this,
-  --                     have free_in_prop x (spec.subst_env (σ₂[g↦value.func g fx R S e σ₂]) R).to_prop, from this,
-  --                     have x ≠ g ∧ free_in_prop x (spec.subst_env σ₂ R).to_prop, from free_of_subst_env_spec this,
-  --                     have x_neq_g: x ≠ g, from this.left,
-  --                     have x_free_in_sR: free_in_prop x (spec.subst_env σ₂ R).to_prop, from this.right,
-  --                     have x_free_in_R: x ∈ FV R.to_prop, from free_of_subst_env x_free_in_sR,
-  --                     have x ∈ FV Q₂ ∪ {g, fx}, from set.mem_of_mem_of_subset x_free_in_R R_fv,
-  --                     have x ∈ FV Q₂ ∨ x ∈ {g, fx}, from set.mem_or_mem_of_mem_union this,
-  --                     or.elim this (
-  --                       assume : x ∈ FV Q₂,
-  --                       have ¬ free_in_prop x (spec.subst_env σ₂ R).to_prop,
-  --                       from not_free_of_subst_env σ₂_verified this R,
-  --                       show ∃v, σ₁ x = some v, from absurd x_free_in_sR this
-  --                     ) (
-  --                       assume : x ∈ {g, fx},
-  --                       have (x = g) ∨ (x = fx), from mem_of_2set this,
-  --                       or.elim this (
-  --                         assume : x = g,
-  --                         show ∃v, σ₁ x = some v, from absurd this x_neq_g
-  --                       ) (
-  --                         assume : x = fx,
-  --                         show ∃v, σ₁ x = some v, from absurd this x_neq_fx
-  --                       )
-  --                     )
-  --                   )
-  --                   (
-  --                     assume x_free_in_pre: free_in_prop x (prop.pre f fx),
-  --                     show ∃v, σ₁ x = some v, by begin
-  --                       cases x_free_in_pre,
-  --                       case free_in_prop.pre₁ x_free_in_f {
-  --                         have : (f = x), from (free_in_term.var.inv x_free_in_f).symm,
-  --                         contradiction
-  --                       },
-  --                       case free_in_prop.pre₂ x_free_in_fx {
-  --                         have : (x = fx), from (free_in_term.var.inv x_free_in_fx),
-  --                         contradiction
-  --                       }
-  --                     end
-  --                   )
-  --                 )
-  --                 (
-  --                   assume : free_in_prop x (prop.implies (R'.to_prop && prop.post f fx) S'.to_prop),
-  --                   or.elim (free_in_prop.implies.inv this) (
-  --                     assume : free_in_prop x (R'.to_prop && prop.post f fx),
-  --                     or.elim (free_in_prop.and.inv this) (
-  --                       assume : free_in_prop x R'.to_prop,
-  --                       have x ≠ g ∧ free_in_prop x (spec.subst_env σ₂ R).to_prop, from free_of_subst_env_spec this,
-  --                       have x_neq_g: x ≠ g, from this.left,
-  --                       have x_free_in_sR: free_in_prop x (spec.subst_env σ₂ R).to_prop, from this.right,
-  --                       have x_free_in_R: x ∈ FV R.to_prop, from free_of_subst_env x_free_in_sR,
-  --                       have x ∈ FV Q₂ ∪ {g, fx}, from set.mem_of_mem_of_subset x_free_in_R R_fv,
-  --                       have x ∈ FV Q₂ ∨ x ∈ {g, fx}, from set.mem_or_mem_of_mem_union this,
-  --                       or.elim this (
-  --                         assume : x ∈ FV Q₂,
-  --                         have ¬ free_in_prop x (spec.subst_env σ₂ R).to_prop,
-  --                         from not_free_of_subst_env σ₂_verified this R,
-  --                         show ∃v, σ₁ x = some v, from absurd x_free_in_sR this
-  --                       ) (
-  --                         assume : x ∈ {g, fx},
-  --                         have (x = g) ∨ (x = fx), from mem_of_2set this,
-  --                         or.elim this (
-  --                           assume : x = g,
-  --                           show ∃v, σ₁ x = some v, from absurd this x_neq_g
-  --                         ) (
-  --                           assume : x = fx,
-  --                           show ∃v, σ₁ x = some v, from absurd this x_neq_fx
-  --                         )
-  --                       )
-  --                     ) (
-  --                       assume : free_in_prop x (prop.post f fx),
-  --                       have free_in_term x f ∨ free_in_term x fx, from free_in_prop.post.inv this,
-  --                       or.elim this (
-  --                         assume : free_in_term x f,
-  --                         have x = f, from free_in_term.var.inv this,
-  --                         show ∃v, σ₁ x = some v, from absurd this f_is_not_x.symm 
-  --                       ) (
-  --                         assume : free_in_term x fx,
-  --                         have x = fx, from free_in_term.var.inv this,
-  --                         show ∃v, σ₁ x = some v, from absurd this x_neq_fx
-  --                       )
-  --                     )
-  --                   ) (
-  --                     assume : free_in_prop x S'.to_prop,
-  --                     have x ≠ g ∧ free_in_prop x (spec.subst_env σ₂ S).to_prop, from free_of_subst_env_spec this,
-  --                     have x_neq_g: x ≠ g, from this.left,
-  --                     have x_free_in_sS: free_in_prop x (spec.subst_env σ₂ S).to_prop, from this.right,
-  --                     have x_free_in_S: x ∈ FV S.to_prop, from free_of_subst_env x_free_in_sS,
-  --                     have x ∈ FV Q₂ ∪ {g, fx}, from set.mem_of_mem_of_subset x_free_in_S S_fv,
-  --                     have x ∈ FV Q₂ ∨ x ∈ {g, fx}, from set.mem_or_mem_of_mem_union this,
-  --                     or.elim this (
-  --                       assume : x ∈ FV Q₂,
-  --                       have ¬ free_in_prop x (spec.subst_env σ₂ S).to_prop,
-  --                       from not_free_of_subst_env σ₂_verified this S,
-  --                       show ∃v, σ₁ x = some v, from absurd x_free_in_sS this
-  --                     ) (
-  --                       assume : x ∈ {g, fx},
-  --                       have (x = g) ∨ (x = fx), from mem_of_2set this,
-  --                       or.elim this (
-  --                         assume : x = g,
-  --                         show ∃v, σ₁ x = some v, from absurd this x_neq_g
-  --                       ) (
-  --                         assume : x = fx,
-  --                         show ∃v, σ₁ x = some v, from absurd this x_neq_fx
-  --                       )
-  --                     )
-  --                   )
-  --                 )
-  --               }
-  --             end
-  --           )
-  --         )
-  --       )
-  --       (
-  --         assume x_free_in_func: free_in_prop x (f ≡ value.func g fx R S e σ₂),
-  --         show ∃v, σ₁ x = some v, by begin
-  --           cases x_free_in_func,
-  --           case free_in_prop.term x_free_in_eq {
-  --             cases x_free_in_eq,
-  --             case free_in_term.binop₁ free_in_f {
-  --               have f_is_x: (f = x), from (free_in_term.var.inv free_in_f).symm,
-  --               contradiction
-  --             },
-  --             case free_in_term.binop₂ free_in_func {
-  --               cases free_in_func
-  --             }
-  --           }
-  --         end
-  --       )
-  --     )
-  --   }
-  -- end
+  assume env_verified: ⊢ σ: P,
+  assume x_free_in_P: x ∈ FV P,
+  begin
+    induction env_verified,
+    case env.vcgen.empty {
+      cases x_free_in_P,
+      case free_in_prop.term x_free_in_true {
+        cases x_free_in_true
+      }
+    },
+    case env.vcgen.tru σ' x' Q _ σ'_verified ih {
+      show ∃v, σ'[x'↦value.true] x = some v, from val_of_free_in_env_value σ'_verified x_free_in_P ih
+    },
+    case env.vcgen.fls σ' x' Q _ σ'_verified ih {
+      show ∃v, σ'[x'↦value.false] x = some v, from val_of_free_in_env_value σ'_verified x_free_in_P ih
+    },
+    case env.vcgen.num n σ' x' Q _ σ'_verified ih { from
+      show ∃v, σ'[x'↦value.num n] x = some v, from val_of_free_in_env_value σ'_verified x_free_in_P ih
+    },
+    case env.vcgen.func σ₁ σ₂ f g fx R S e Q₁ Q₂ Q₃ _ σ₁_verified σ₂_verified R_fv S_fv func_verified S_valid {
+      show ∃v, σ₁[f↦value.func g fx R S e σ₂] x = some v, from val_of_free_in_env_value σ₁_verified x_free_in_P ih_1
+    }
+  end
+
+lemma val_of_free_in_hist_env {H: list call} {σ: env} {P: prop} {x: var}:
+                              (⊢ σ : P) → x ∈ FV (↑H && P) → ∃v, σ x = some v :=
+  assume σ_verified: ⊢ σ : P,
+  assume x_free_in_H_P: x ∈ FV (↑H && P),
+  have free_in_prop x H ∨ free_in_prop x P, from free_in_prop.and.inv x_free_in_H_P,
+  have x ∈ FV P, from or.elim this.symm id (
+    assume : free_in_prop x H,
+    show free_in_prop x P, from absurd this (call_history_closed H x)
+  ),
+  show ∃v, σ x = some v, from val_of_free_in_env σ_verified this
 
 lemma simple_equality_valid {σ: env} {x: var} {v: value}:
   x ∉ σ → (σ[x↦v]) ⊨ (prop.term (x ≡ v)).erased :=
@@ -658,62 +251,19 @@ lemma env_translation_erased_valid {P: prop} {σ: env}: (⊢ σ: P) → σ ⊨ P
       show (σ'[x'↦value.true]) ⊨ prop.erased (Q && (x' ≡ value.true)),
       from simple_equality_env_valid σ'_verified x_not_free_in_σ' ih
     },
-    case env.vcgen.fls σ' x' Q x_not_free_in_σ' σ'_verified ih { from
+    case env.vcgen.fls σ' x' Q x_not_free_in_σ' σ'_verified ih {
       show (σ'[x'↦value.false]) ⊨ prop.erased (Q && (x' ≡ value.false)),
       from simple_equality_env_valid σ'_verified x_not_free_in_σ' ih
     },
-    case env.vcgen.num n σ' x' Q x_not_free_in_σ' σ'_verified ih { from
+    case env.vcgen.num n σ' x' Q x_not_free_in_σ' σ'_verified ih {
       show (σ'[x'↦value.num n]) ⊨ prop.erased (Q && (x' ≡ value.num n)),
       from simple_equality_env_valid σ'_verified x_not_free_in_σ' ih
     },
     case env.vcgen.func σ₁ σ₂ f g gx R S e Q₁ Q₂ Q₃
-      x_not_free_in_σ₁ σ₁_verified σ₂_verified R_fv S_fv func_verified S_valid ih₁ ih₂ { from (
-      have h1: (σ₁[f↦value.func g gx R S e σ₂]) ⊨ prop.erased (Q₁ && (f ≡ value.func g gx R S e σ₂)),
-      from simple_equality_env_valid σ₁_verified x_not_free_in_σ₁ ih₁,
-
-
-      have h2: (σ₁[f↦value.func g gx R S e σ₂]) ⊨ 
-            prop.erased (spec.func ↑f gx (spec.subst_env (σ₂[g↦value.func g gx R S e σ₂]) R)
-                                         (spec.subst_env (σ₂[g↦value.func g gx R S e σ₂]) S)), from sorry,
-      have h3: ⊨ (
-           (vc.subst_env (σ₁[f↦value.func g gx R S e σ₂])
-            (prop.erased (Q₁ && ↑(↑f ≡ ↑(value.func g gx R S e σ₂)))))
-        && (vc.subst_env (σ₁[f↦value.func g gx R S e σ₂])
-            (prop.erased ↑(spec.func ↑f gx (spec.subst_env (σ₂[g↦value.func g gx R S e σ₂]) R)
-                                           (spec.subst_env (σ₂[g↦value.func g gx R S e σ₂]) S))))),
-      from valid.and.mp ⟨h1, h2⟩,
-      have
-        vc.subst_env (σ₁[f↦value.func g gx R S e σ₂])
-           ((prop.erased (Q₁ && ↑(↑f ≡ ↑(value.func g gx R S e σ₂))))
-         && (prop.erased ↑(spec.func ↑f gx (spec.subst_env (σ₂[g↦value.func g gx R S e σ₂]) R)
-                                           (spec.subst_env (σ₂[g↦value.func g gx R S e σ₂]) S))))
-        =  (vc.subst_env (σ₁[f↦value.func g gx R S e σ₂])
-            (prop.erased (Q₁ && ↑(↑f ≡ ↑(value.func g gx R S e σ₂)))))
-        && (vc.subst_env (σ₁[f↦value.func g gx R S e σ₂])
-            (prop.erased ↑(spec.func ↑f gx (spec.subst_env (σ₂[g↦value.func g gx R S e σ₂]) R)
-                                           (spec.subst_env (σ₂[g↦value.func g gx R S e σ₂]) S)))),
-      from vc.subst_env.and,
-      have h4: (σ₁[f↦value.func g gx R S e σ₂]) ⊨ 
-           ((prop.erased (Q₁ && ↑(↑f ≡ ↑(value.func g gx R S e σ₂))))
-         && (prop.erased ↑(spec.func ↑f gx (spec.subst_env (σ₂[g↦value.func g gx R S e σ₂]) R)
-                                           (spec.subst_env (σ₂[g↦value.func g gx R S e σ₂]) S)))),
-      from this.symm ▸ h3,
-      have prop.erased (prop.and (Q₁
-                        && ↑(↑f ≡ ↑(value.func g gx R S e σ₂)))
-                        ↑(spec.func ↑f gx (spec.subst_env (σ₂[g↦value.func g gx R S e σ₂]) R)
-                                             (spec.subst_env (σ₂[g↦value.func g gx R S e σ₂]) S)))
-         = prop.erased (Q₁
-                        && ↑(↑f ≡ ↑(value.func g gx R S e σ₂)))
-        && prop.erased ↑(spec.func ↑f gx (spec.subst_env (σ₂[g↦value.func g gx R S e σ₂]) R)
-                                         (spec.subst_env (σ₂[g↦value.func g gx R S e σ₂]) S)),
-      by unfold prop.erased,
-      show (σ₁[f↦value.func g gx R S e σ₂]) ⊨ 
-           prop.erased (Q₁
-                        && ↑(↑f ≡ ↑(value.func g gx R S e σ₂))
-                        && ↑(spec.func ↑f gx (spec.subst_env (σ₂[g↦value.func g gx R S e σ₂]) R)
-                                             (spec.subst_env (σ₂[g↦value.func g gx R S e σ₂]) S))),
-      from this.symm ▸ h4
-    )}
+      x_not_free_in_σ₁ σ₁_verified σ₂_verified R_fv S_fv func_verified S_valid ih₁ ih₂ {
+      show (σ₁[f↦value.func g gx R S e σ₂]) ⊨ prop.erased (Q₁ && (f ≡ value.func g gx R S e σ₂)),
+      from simple_equality_env_valid σ₁_verified x_not_free_in_σ₁ ih₁
+    }
   end
 
 lemma env_translation_valid {H: list call} {P: prop} {σ: env}:
@@ -723,117 +273,244 @@ lemma env_translation_valid {H: list call} {P: prop} {σ: env}:
   have h1: σ ⊨ prop.instantiated ↑H, from h_valid σ,
   have σ ⊨ P.erased, from env_translation_erased_valid env_verified,
   have h2: σ ⊨ P.instantiated, from instantiated_of_erased this,
-  have σ ⊨ (↑H && P).instantiated, from instantiated_and h1 h2,
+  have σ ⊨ (prop.instantiated ↑H && P.instantiated), from valid_env.and h1 h2,
+  have σ ⊨ (↑H && P).instantiated, from instantiated_and this,
   show σ ⊨ (↑H && P).instantiated_n, from instantiated_n_of_instantiated this
 
-lemma exp.progress{H: list call} {P: prop} {Q: propctx} {e: exp} {σ: env}:
-                  ⟪H⟫ → (⊢ σ: P) → (H && P ⊢ e: Q) → is_return (σ, e) ∨ ∃c s', (σ, e) ⟶ c, s'
+lemma consequent_of_H_P {H: list call} {σ: env} {P Q: prop}:
+  ⟪H⟫ → (⊢ σ: P) → ⟪prop.implies (↑H && P) Q⟫ → no_instantiations Q → σ ⊨ Q.erased :=
+  assume h_valid: ⟪H⟫,
+  assume env_verified: (⊢ σ : P),
+  assume impl_vc: ⟪prop.implies (↑H && P) Q⟫,
+  assume : no_instantiations Q,
+  have h1: (prop.implies (↑H && P) Q).instantiated = vc.or (↑H && P).not.instantiated Q.erased,
+  from or_dist_of_no_instantiations this,
+  have h2: (↑H && P).not.instantiated = (↑H && P).instantiated_n.not, from not_dist_instantiated,
+  have σ ⊨ (prop.implies (↑H && P) Q).instantiated, from impl_vc σ,
+  have σ ⊨ vc.or (↑H && P).instantiated_n.not Q.erased, from h2 ▸ h1 ▸ this,
+  have h4: σ ⊨ vc.implies (↑H && P).instantiated_n Q.erased, from this,
+  have σ ⊨ (↑H && P).instantiated_n, from env_translation_valid h_valid env_verified,
+  show σ ⊨ Q.erased, from valid_env.mp h4 this
+
+lemma env_translation_call_valid {H: list call} {P: prop} {σ: env} {f x: var}:
+  ⟪H⟫ → (⊢ σ: P) → σ ⊨ (↑H && P && prop.call f x).instantiated_n :=
+  assume h_valid: ⟪H⟫,
+  assume env_verified: (⊢ σ : P),
+  have h1: σ ⊨ prop.instantiated ↑H, from h_valid σ,
+  have σ ⊨ P.erased, from env_translation_erased_valid env_verified,
+  have h2: σ ⊨ P.instantiated, from instantiated_of_erased this,
+  have σ ⊨ (prop.instantiated ↑H && P.instantiated), from valid_env.and h1 h2,
+  have h3: σ ⊨ (↑H && P).instantiated, from instantiated_and this,
+  have h4: ⊨ value.true, from valid.tru,
+  have term.subst_env σ value.true = value.true, from term.subst_env.value,
+  have h5: ⊨ term.subst_env σ value.true, from this.symm ▸ h4,
+  have vc.subst_env σ value.true = vc.term (term.subst_env σ value.true), from vc.subst_env.term,
+  have h6: σ ⊨ value.true, from this.symm ▸ h5,
+  have (prop.call f x).erased = vc.term value.true, by unfold prop.erased,
+  have σ ⊨ (prop.call f x).erased, from this.symm ▸ h6,
+  have σ ⊨ (prop.call f x).instantiated, from instantiated_of_erased this,
+  have σ ⊨ ((↑H && P).instantiated && (prop.call f x).instantiated), from valid_env.and h3 this,
+  have σ ⊨ (↑H && P && prop.call f x).instantiated, from instantiated_and this,
+  show σ ⊨ (↑H && P && prop.call f x).instantiated_n, from instantiated_n_of_instantiated this
+
+lemma consequent_of_H_P_call {H: list call} {σ: env} {P Q: prop} {f x: var}:
+  ⟪H⟫ → (⊢ σ: P) → ⟪prop.implies (↑H && P && prop.call f x) Q⟫ → no_instantiations Q → σ ⊨ Q.erased :=
+  assume h_valid: ⟪H⟫,
+  assume env_verified: (⊢ σ : P),
+  assume impl_vc: ⟪prop.implies (↑H && P && prop.call f x) Q⟫,
+  assume : no_instantiations Q,
+  have h1: (prop.implies (↑H && P && prop.call f x) Q).instantiated
+         = vc.or (↑H && P && prop.call f x).not.instantiated Q.erased,
+  from or_dist_of_no_instantiations this,
+  have h2: (↑H && P && prop.call f x).not.instantiated = (↑H && P && prop.call f x).instantiated_n.not,
+  from not_dist_instantiated,
+  have σ ⊨ (prop.implies (↑H && P && prop.call f x) Q).instantiated, from impl_vc σ,
+  have σ ⊨ vc.or (↑H && P && prop.call f x).instantiated_n.not Q.erased, from h2 ▸ h1 ▸ this,
+  have h4: σ ⊨ vc.implies (↑H && P && prop.call f x).instantiated_n Q.erased, from this,
+  have σ ⊨ (↑H && P && prop.call f x).instantiated_n, from env_translation_call_valid h_valid env_verified,
+  show σ ⊨ Q.erased, from valid_env.mp h4 this
+
+lemma exp.progress {H: list call} {P: prop} {Q: propctx} {e: exp} {σ: env}:
+                   ⟪H⟫ → (⊢ σ: P) → (H && P ⊢ e: Q) → is_value (σ, e) ∨ ∃c s', (σ, e) ⟶ c, s'
 :=
   assume h_valid: ⟪H⟫,
   assume env_verified: (⊢ σ : P),
   assume e_verified: (H && P ⊢ e : Q),
-  show is_return (σ, e) ∨ ∃c s', (σ, e) ⟶ c, s', from begin
+  show is_value (σ, e) ∨ ∃c s', (σ, e) ⟶ c, s', from begin
     cases e_verified,
     case exp.vcgen.tru x e' { from
       let s: stack := (σ, lett x = true in e') in
       have s ⟶ none, (σ[x↦value.true], e'), from step.tru,
       have ∃c s', s ⟶ c, s', from exists.intro none (exists.intro (σ[x↦value.true], e') this),
-      show is_return s ∨ ∃c s', s ⟶ c, s', from or.inr this
+      show is_value s ∨ ∃c s', s ⟶ c, s', from or.inr this
     },
     case exp.vcgen.fals x e' { from
       let s: stack := (σ, letf x = false in e') in
       have s ⟶ none, (σ[x↦value.false], e'), from step.fals,
       have ∃c s', s ⟶ c, s', from exists.intro none (exists.intro (σ[x↦value.false], e') this),
-      show is_return s ∨ ∃c s', s ⟶ c, s', from or.inr this
+      show is_value s ∨ ∃c s', s ⟶ c, s', from or.inr this
     },
     case exp.vcgen.num x n e' { from
       let s: stack := (σ, letn x = n in e') in
       have s ⟶ none, (σ[x↦value.num n], e'), from step.num,
       have ∃c s', s ⟶ c, s', from exists.intro none (exists.intro (σ[x↦value.num n], e') this),
-      show is_return s ∨ ∃c s', s ⟶ c, s', from or.inr this
+      show is_value s ∨ ∃c s', s ⟶ c, s', from or.inr this
     },
     case exp.vcgen.func f x R S e₁ e₂ { from
       let s: stack := (σ, letf f[x] req R ens S {e₁} in e₂) in
       have s ⟶ none, (σ[f↦value.func f x R S e₁ σ], e₂), from step.closure,
       have ∃c s', s ⟶ c, s', from exists.intro none (exists.intro (σ[f↦value.func f x R S e₁ σ], e₂) this),
-      show is_return s ∨ ∃c s', s ⟶ c, s', from or.inr this
+      show is_value s ∨ ∃c s', s ⟶ c, s', from or.inr this
     },
-    case exp.vcgen.unop op x y e' Q' x_free_in_P _ e'_verified pre_valid { from
+    case exp.vcgen.unop op x y e' Q' x_free_in_P _ e'_verified vc_valid { from
       let s: stack := (σ, letop y = op[x] in e') in
-      have free_in_prop x H ∨ free_in_prop x P, from free_in_prop.and.inv x_free_in_P,
-      have x ∈ FV P, from or.elim this.symm id (
-        assume : free_in_prop x H,
-        show free_in_prop x P, from absurd this (call_history_closed H x)
-      ),
-      have ∃v, σ x = some v, from val_of_free_in_env env_verified this,
-      let ⟨v, env_has_x⟩ := this in
+      let ⟨v, env_has_x⟩ := (val_of_free_in_hist_env env_verified x_free_in_P) in
       have no_instantiations (prop.pre₁ op x), from no_instantiations.pre₁,
-      have h1: (prop.implies (↑H && P) (prop.pre₁ op x)).instantiated
-              = vc.or (↑H && P).not.instantiated (prop.pre₁ op x).erased,
-      from or_dist_of_no_instantiations this,
-      have h2: (prop.pre₁ op x).erased = (vc.pre₁ op x), by unfold prop.erased,
-      have h3: (↑H && P).not.instantiated = (↑H && P).instantiated_n.not, from not_dist_instantiated,
-      have σ ⊨ (prop.implies (↑H && P) (prop.pre₁ op x)).instantiated, from pre_valid σ,
-      have σ ⊨ vc.or (↑H && P).instantiated_n.not (vc.pre₁ op x), from h3 ▸ h2 ▸ h1 ▸ this,
-      have h4: σ ⊨ vc.implies (↑H && P).instantiated_n (vc.pre₁ op x), from this,
-      have σ ⊨ (↑H && P).instantiated_n, from env_translation_valid h_valid env_verified,
-      have σ ⊨ vc.pre₁ op x, from valid.mp_env h4 this,
-      have h5: ⊨ vc.subst_env σ (vc.pre₁ op x), from this,
+      have σ ⊨ (prop.pre₁ op x).erased, from consequent_of_H_P h_valid env_verified vc_valid this,
+      have h1: ⊨ vc.subst_env σ (vc.pre₁ op x), from this,
       have vc.subst_env σ (vc.pre₁ op x) = vc.pre₁ op (term.subst_env σ x), from vc.subst_env.pre₁,
-      have ⊨ vc.pre₁ op (term.subst_env σ x), from this ▸ h5,
+      have ⊨ vc.pre₁ op (term.subst_env σ x), from this ▸ h1,
       have x_from_env: term.subst_env σ x = v, from (term.subst_env.var.right v).mp env_has_x,
       have ⊨ vc.pre₁ op v, from x_from_env ▸ this,
-      have (∃v', unop.apply op v = some v'), from valid.pre₁.inv this,
+      have (∃v', unop.apply op v = some v'), from valid.pre₁.mpr this,
       let ⟨v', op_v_is_v'⟩ := this in
       have s ⟶ none, (σ[y↦v'], e'), from step.unop env_has_x op_v_is_v',
       have ∃c s', s ⟶ c, s', from exists.intro none (exists.intro (σ[y↦v'], e') this),
-      show is_return s ∨ ∃c s', s ⟶ c, s', from or.inr this
+      show is_value s ∨ ∃c s', s ⟶ c, s', from or.inr this
     },
-
-
-    case exp.vcgen.return a x { from
+    case exp.vcgen.binop op x y z e' Q' x_free_in_P y_free_in_P _ e'_verified vc_valid { from
+      let s: stack := (σ, letop2 z = op[x,y] in e') in
+      let ⟨vx, env_has_x⟩ := (val_of_free_in_hist_env env_verified x_free_in_P) in
+      let ⟨vy, env_has_y⟩ := (val_of_free_in_hist_env env_verified y_free_in_P) in
+      have no_instantiations (prop.pre₂ op x y), from no_instantiations.pre₂,
+      have σ ⊨ (prop.pre₂ op x y).erased, from consequent_of_H_P h_valid env_verified vc_valid this,
+      have h1: ⊨ vc.subst_env σ (vc.pre₂ op x y), from this,
+      have vc.subst_env σ (vc.pre₂ op x y) = vc.pre₂ op (term.subst_env σ x) (term.subst_env σ y),
+      from vc.subst_env.pre₂,
+      have h2: ⊨ vc.pre₂ op (term.subst_env σ x) (term.subst_env σ y), from this ▸ h1,
+      have term.subst_env σ x = vx, from (term.subst_env.var.right vx).mp env_has_x,
+      have h3: ⊨ vc.pre₂ op vx (term.subst_env σ y), from this ▸ h2,
+      have term.subst_env σ y = vy, from (term.subst_env.var.right vy).mp env_has_y,
+      have ⊨ vc.pre₂ op vx vy, from this ▸ h3,
+      have (∃v', binop.apply op vx vy = some v'), from valid.pre₂.mpr this,
+      let ⟨v', op_v_is_v'⟩ := this in
+      have s ⟶ none, (σ[z↦v'], e'), from step.binop env_has_x env_has_y op_v_is_v',
+      have ∃c s', s ⟶ c, s', from exists.intro none (exists.intro (σ[z↦v'], e') this),
+      show is_value s ∨ ∃c s', s ⟶ c, s', from or.inr this
+    },
+    case exp.vcgen.app y f x e' Q' f_free_in_P x_free_in_P _ e'_verified vc_valid { from
+      let s: stack := (σ, letapp y = f [x] in e') in
+      let ⟨vf, env_has_f⟩ := (val_of_free_in_hist_env env_verified f_free_in_P) in
+      let ⟨vx, env_has_x⟩ := (val_of_free_in_hist_env env_verified x_free_in_P) in
+      have h1: no_instantiations (term.unop unop.isFunc f), from no_instantiations.term,
+      have h2: no_instantiations (prop.pre f x), from no_instantiations.pre,
+      have no_instantiations (↑(term.unop unop.isFunc f) && prop.pre f x), from no_instantiations.and h1 h2,
+      have h3: σ ⊨ (↑(term.unop unop.isFunc f) && prop.pre f x).erased,
+      from consequent_of_H_P_call h_valid env_verified vc_valid this,
+      have (prop.and (prop.term (term.unop unop.isFunc f)) (prop.pre f x)).erased
+         = (prop.term (term.unop unop.isFunc f)).erased && (prop.pre f x).erased, by unfold prop.erased,
+      have σ ⊨ ((prop.term (term.unop unop.isFunc f)).erased && (prop.pre f x).erased), from this ▸ h3,
+      have h4: ⊨ vc.subst_env σ ((prop.term (term.unop unop.isFunc f)).erased && (prop.pre f x).erased), from this,
+      have vc.subst_env σ ((prop.term (term.unop unop.isFunc f)).erased && (prop.pre f x).erased)
+         = vc.subst_env σ ((prop.term (term.unop unop.isFunc f)).erased) && vc.subst_env σ ((prop.pre f x).erased),
+      from vc.subst_env.and,
+      have ⊨ (vc.subst_env σ ((prop.term (term.unop unop.isFunc f)).erased) && vc.subst_env σ ((prop.pre f x).erased)),
+      from this ▸ h4,
+      have h5: σ ⊨ (prop.term (term.unop unop.isFunc f)).erased, from (valid.and.mpr this).left,
+      have (prop.term (term.unop unop.isFunc f)).erased = vc.term (term.unop unop.isFunc f),
+      by unfold prop.erased,
+      have h6: σ ⊨ vc.term (term.unop unop.isFunc f), from this ▸ h5,
+      have vc.subst_env σ (vc.term (term.unop unop.isFunc f)) = vc.term (term.subst_env σ (term.unop unop.isFunc f)),
+      from vc.subst_env.term,
+      have h7: ⊨ vc.term (term.subst_env σ (term.unop unop.isFunc f)), from this ▸ h6,
+      have term.subst_env σ (term.unop unop.isFunc f) = term.unop unop.isFunc (term.subst_env σ f),
+      from term.subst_env.unop,
+      have h8: ⊨ vc.term (term.unop unop.isFunc (term.subst_env σ f)), from this ▸ h7,
+      have term.subst_env σ f = vf, from (term.subst_env.var.right vf).mp env_has_f,
+      have ⊨ term.unop unop.isFunc vf, from this ▸ h8,
+      have ⊨ (term.unop unop.isFunc vf ≡ value.true), from valid.eq.true.mpr this,
+      have unop.apply unop.isFunc vf = some value.true, from valid.unop.mpr this,
+      have ∃(g gx: var) (gR gS: spec) (ge: exp) (gσ: env), vf = value.func g gx gR gS ge gσ,
+      from unop.isFunc.inv this,
+      let ⟨g, gx, gR, gS, ge, gσ, vf_is_g⟩ := this in
+      have some_vf_is_g: some vf = ↑(value.func g gx gR gS ge gσ), from some.inj.inv vf_is_g,
+      have σ f = value.func g gx gR gS ge gσ, from eq.trans env_has_f some_vf_is_g,
+      let s': stack := (gσ[g↦value.func g gx gR gS ge gσ][gx↦vx], ge) · [σ, let y = f[x] in e'] in
+      have s ⟶ none, s', from step.app this env_has_x,
+      have ∃c s', s ⟶ c, s', from exists.intro none (exists.intro s' this),
+      show is_value s ∨ ∃c s', s ⟶ c, s', from or.inr this
+    },
+    case exp.vcgen.ite x e₂ e₁ Q₁ Q₂ x_free_in_P _ _ vc_valid { from
+      let s: stack := (σ, exp.ite x e₁ e₂) in
+      let ⟨v, env_has_x⟩ := (val_of_free_in_hist_env env_verified x_free_in_P) in
+      have no_instantiations (term.unop unop.isBool x), from no_instantiations.term,
+      have h1: σ ⊨ (prop.term (term.unop unop.isBool x)).erased,
+      from consequent_of_H_P h_valid env_verified vc_valid this,
+      have (prop.term (term.unop unop.isBool x)).erased = vc.term (term.unop unop.isBool x),
+      by unfold prop.erased,
+      have h2: σ ⊨ vc.term (term.unop unop.isBool x), from this ▸ h1,
+      have vc.subst_env σ (vc.term (term.unop unop.isBool x)) = vc.term (term.subst_env σ (term.unop unop.isBool x)),
+      from vc.subst_env.term,
+      have h3: ⊨ vc.term (term.subst_env σ (term.unop unop.isBool x)), from this ▸ h2,
+      have term.subst_env σ (term.unop unop.isBool x) = term.unop unop.isBool (term.subst_env σ x),
+      from term.subst_env.unop,
+      have h4: ⊨ vc.term (term.unop unop.isBool (term.subst_env σ x)), from this ▸ h3,
+      have term.subst_env σ x = v, from (term.subst_env.var.right v).mp env_has_x,
+      have ⊨ term.unop unop.isBool v, from this ▸ h4,
+      have ⊨ (term.unop unop.isBool v ≡ value.true), from valid.eq.true.mpr this,
+      have unop.apply unop.isBool v = some value.true, from valid.unop.mpr this,
+      have (v = value.true) ∨ (v = value.false), from unop.isBool.inv this,
+      or.elim this (
+        assume : v = value.true,
+        have some v = some value.true, from some.inj.inv this,
+        have σ x = value.true, from eq.trans env_has_x this,
+        have s ⟶ none, (σ, e₁), from step.ite_true this,
+        have ∃c s', s ⟶ c, s', from exists.intro none (exists.intro (σ, e₁) this),
+        show is_value s ∨ ∃c s', s ⟶ c, s', from or.inr this
+      ) (
+        assume : v = value.false,
+        have some v = some value.false, from some.inj.inv this,
+        have σ x = value.false, from eq.trans env_has_x this,
+        have s ⟶ none, (σ, e₂), from step.ite_false this,
+        have ∃c s', s ⟶ c, s', from exists.intro none (exists.intro (σ, e₂) this),
+        show is_value s ∨ ∃c s', s ⟶ c, s', from or.inr this
+      )
+    },
+    case exp.vcgen.return x x_free_in_P { from
       let s: stack := (σ, exp.return x) in
       have s_is_return: s = (σ, exp.return x), from rfl,
-      have is_return_s: is_return s = (∃(σ': env) (x': var), s = (σ', exp.return x')), by unfold is_return,
-      have (∃(σ': env) (x': var), s = (σ', exp.return x')), from exists.intro σ (exists.intro x s_is_return),
-      have is_return s, from is_return_s ▸ this,
-      show is_return s ∨ ∃c s', s ⟶ c, s', from or.inl this
+      let ⟨v, env_has_x⟩ := (val_of_free_in_hist_env env_verified x_free_in_P) in
+      have is_value_s: is_value s = (∃(σ': env) (x': var) (v: value), s = (σ', exp.return x') ∧ (σ' x' = v)),
+      by unfold is_value,
+      have (∃(σ': env) (x': var) (v: value), s = (σ', exp.return x') ∧ (σ' x' = v)),
+      from exists.intro σ (exists.intro x (exists.intro v ⟨s_is_return, env_has_x⟩)),
+      have is_value s, from is_value_s ▸ this,
+      show is_value s ∨ ∃c s', s ⟶ c, s', from or.inl this
     }
   end
 
-theorem progress(H: list call) (s: stack): ⟪H⟫ → (H ⊩ s) → is_return s ∨ ∃c s', s ⟶ c, s'
+theorem progress(H: list call) (s: stack): ⟪H⟫ → (H ⊩ s) → is_value s ∨ ∃c s', s ⟶ c, s'
 :=
   assume h_valid: ⟪H⟫,
   assume s_verified: H ⊩ s,
   begin
     induction s_verified,
     case stack.vcgen.top σ e Q P H env_verified e_verified { from
-      show is_return (σ, e) ∨ ∃c s', (σ, e) ⟶ c, s', from exp.progress h_valid env_verified e_verified
+      show is_value (σ, e) ∨ ∃c s', (σ, e) ⟶ c, s', from exp.progress h_valid env_verified e_verified
     },
     case stack.vcgen.cons H P s' σ σ' f g x y gx R S e vₓ Q s'_verified env_verified f_is_func x_is_v _ cont ih { from
       let s := (s' · [σ, let y = f[x] in e]) in
       have s_cons: s = (s' · [σ, let y = f[x] in e]), from rfl,
       (ih h_valid).elim
       ( -- step return
-        assume s'_is_return: is_return s',
-        let ⟨σ₂, z, s'_return⟩ := s'_is_return in
+        assume s'_is_value: is_value s',
+        let ⟨σ₂, z, v, ⟨s'_return, env2_has_z⟩⟩ := s'_is_value in
         have s_return_cons: s = ((σ₂, exp.return z) · [σ, let y = f[x] in e]), from s'_return ▸ s_cons,
-        have H ⊩ (σ₂, exp.return z), from s'_return ▸ s'_verified,
-        have ∃P' Q', (⊢ σ₂: P') ∧ (H && P' ⊢ exp.return z: Q'), from stack.vcgen.top.inv this,
-        let ⟨P', Q', ⟨env2_verified, return_verified⟩⟩ := this in
-        have z ∈ FV (↑H && P'), from exp.vcgen.return.inv return_verified,
-        have free_in_prop z H ∨ free_in_prop z P', from free_in_prop.and.inv this,
-        have z ∈ FV P', from or.elim this.symm id (
-          assume : free_in_prop z H,
-          show free_in_prop z P', from absurd this (call_history_closed H z)
-        ),
-        have ∃v, σ₂ z = some v, from val_of_free_in_env env2_verified this,
-        let ⟨v, env2_has_z⟩ := this in
         have s ⟶ some ⟨g, gx, R, S, e, σ', vₓ, v⟩, (σ[y↦v], e),
         from s_return_cons.symm ▸ (step.return env2_has_z f_is_func x_is_v),
         have ∃s', s ⟶ some ⟨g, gx, R, S, e, σ', vₓ, v⟩, s', from exists.intro (σ[y↦v], e) this,
         have ∃c s', s ⟶ c, s', from exists.intro (some ⟨g, gx, R, S, e, σ', vₓ, v⟩) this,
-        show is_return s ∨ ∃c s', s ⟶ c, s', from or.inr this
+        show is_value s ∨ ∃c s', s ⟶ c, s', from or.inr this
       )
       ( -- step ctx
         assume s'_can_step: ∃c s'', s' ⟶ c, s'',
@@ -841,7 +518,7 @@ theorem progress(H: list call) (s: stack): ⟪H⟫ → (H ⊩ s) → is_return s
         have s ⟶ c, (s'' · [σ, let y = f[x] in e]), from step.ctx s'_steps,
         have ∃s', s ⟶ c, s', from exists.intro (s'' · [σ, let y = f[x] in e]) this,
         have ∃c s', s ⟶ c, s', from exists.intro c this,
-        show is_return s ∨ ∃c s', s ⟶ c, s', from or.inr this
+        show is_value s ∨ ∃c s', s ⟶ c, s', from or.inr this
       )
     }
   end
