preservation.lean
@@ -1,0 +1,5 @@
+import .syntax .notations .logic .evaluation .vcgen
+
+theorem preservation {H: list call} {h: call} {s s': stack}:
+  (H ⊩ s) → (s ⟶ h, s') → (h :: H ⊩ s') ∧ ⟪[h]⟫
+:= sorry
