soundness.lean
@@ -1,0 +1,17 @@
+import .syntax .notations .logic .evaluation .vcgen .progress .preservation
+
+theorem soundness {e: exp} {s: stack}:
+  (list.nil ⊩ (env.empty, e)) → ((env.empty, e) ⟶* s) → (is_value s ∨ ∃s' h, s ⟶ h, s') :=
+  assume initial_verified: (list.nil ⊩ (env.empty, e)),
+  assume stepped_to_s: ((env.empty, e) ⟶* s),
+  begin
+    induction stepped_to_s,
+    case trans_step.rfl s_initial {
+      let H: list call := list.nil,
+      have H_valid: ⟪H⟫, from empty_history_valid,
+      show is_value s_initial ∨ ∃s' h, s_initial ⟶ h, s', from progress H H_valid initial_verified
+    },
+    case trans_step.trans a b c d e f {
+
+    }
+  end
